### 可分离变量的微分方程

$$
\newcommand{\d}{\mathrm d}
\begin{align}
y' &= f(x)g(y) \\
\frac{\d y}{\d x} &= f(x)g(y) \\
\frac{\d y}{g(y)} &= f(x)\d x \\
\int \frac{\d y}{g(y)} &= \int f(x)\d x
\end{align}
$$

例 1  
$$
\newcommand{\d}{\mathrm d}
\begin{align}
\tan x \frac{\d y}{\d x} &= 1 + y \\
\frac{\d y}{\d x} &= \cot x(1 + y) \\
(y \not\equiv -1) \quad \frac{\d y}{1 + y} &= \cot x \, \d x \\
\ln |y + 1| &= \int \cot x \, \d x \\
&= \int \frac{\cos x}{\sin x} \d x \\
&= \int \frac{1}{\sin x} \d (\sin x) \\
&= \ln |\sin x| + C \\
\quad \ln |y + 1| &= \ln |C \sin x| \quad (C := \exp C, C \ne 0) \\
y + 1 &= \pm C \sin x \\
y &= C \sin x - 1 \quad (C := \pm C) \\
(y \equiv - 1) \quad \frac{\d y}{\d x} &= 1 + y = 0 \\
(\implies) \quad y &= C \sin x - 1 \quad (C \in \R)
\end{align}
$$


$$
\newcommand{\d}{\mathrm d}
\begin{align}
y' + f(x)y &= g(x) \\

\frac{\d y}{\d x} &= -f(x)y + g(x) \\

\frac{\d y}{y} &= \left( -f(x) + \frac{g(x)}{y} \right) \d x \\

\ln |y| &=  \int \left( -f(x) + \frac{g(x)}{y} \right) \d x \\

\ln |y| &= - \int f(x) \d x + \int \frac{g(x)}{y} \d x + \ln C \\

y &= e^{ -\int f(x) \d x } \cdot e^{ \int \frac{g(x)}{y} \d x } \cdot C \\

y &= e^{ -\int f(x) \d x } u(x)
\quad \left( u(x) := Ce^{ \int \frac{g(x)}{y} \d x } \right) \\

y' &= -f(x) e^{ -\int f(x) \d x } \cdot u(x) + e^{ -\int f(x) \d x } \cdot u'(x) \\

&= -f(x)y + g(x) \\

g(x) &= e^{ -\int f(x) \d x } \cdot u'(x) \\

u'(x) &= g(x) e^{ \int f(x) \d x } \\

u(x) &= \int g(x)e^{ \int f(x) \d x } + C \\

y &= \boxed{ -e^{ \int f(x) \d x } \left( \int g(x)e^{ \int f(x) \d x } + C \right) } \\

y &= \boxed{ e^{ -\int f(x) \d x } \int g(x)e^{ \int f(x) \d x } + Ce^{ -\int f(x) \d x } } \\

y &= y_0 + e^{ -\int f(x) \d x } \int g(x)e^{ \int f(x) \d x }y 
\end{align}
$$


### 齐次微分方程

$$
\newcommand{\d}{\mathrm d}
\begin{align}
y' &= f \left( \frac{y}{x} \right) \\
\frac{y}{x} &:= u \\
y &= ux \\
\frac{\d y}{\d x} &= \frac{\d u}{\d x} x + u \\
\frac{\d u}{\d x} x + u &= f(u) \\
x \d u &= \d x(f(u) - u) \\
\frac{\d x}{x} &= \frac{\d u}{f(u) - u} \\
\ln |x| &= \int \frac{\d u}{f(u) - u}
\end{align}
$$

### 二阶常系数齐次线性微分方程

$$
\newcommand{\d}{\mathrm d}
\begin{align}
y'' + py' + qy &= 0 \\
r^2e^{rx} + pre^{rx} + qe^{rx} &= 0 \quad (y := e^{rx}) \\
r^2 + pr + q &= 0 \quad (\text{特征方程}) \\
p &= -(r_1 +  r_2) \\
q &= r_1r_2 \\

y'' + -(r_1 + r_2)y' + r_1r_2y &= 0 \\
(y'' - r_2y') - r_1(y' - r_2y) &= 0 \\
(y' - r_2y)' - r_1(y' - r_2y) &= 0 \\

u' - r_1u &= 0 \quad (u := y' - r_2y) \\
u' &= r_1u \\
u &= C_1e^{r_1x} \\
y' - r_2y &= C_1e^{r_1x} \\

y &= e^{-(-r_2x)} \left( \int e^{-r_2x} \cdot C_1e^{r_1x} \d x + C_2 \right) \\
&= e^{r_2x} \left( C_1 \int e^{(r_1 - r_2)x} \d x + C_2 \right) \\

(r_1 = r_2 \in \R) \quad &= e^{r_2x}(C_1x + C_2) \\
&= e^{-\frac12 px}(C_1x + C_2) \\

(r_1 \neq r_2 \in \R) \quad &= e^{r_2x} \cdot \left( \frac{C_1}{r_1 - r_2} \cdot e^{(r_1 - r_2)x} + C_2 \right) \\
&= e^{r_2x} \cdot \left( C_1e^{(r_1 - r_2)x} + C_2 \right) \quad \left( C_1 := \frac{C_1}{r_1 - r_2} \right) \\
&= C_1e^{r_1x} + C_2e^{r_2}x \\
&= C_1e^{\frac{-p + \sqrt{p^2 - 4q}}{2}x} + C_2e^{\frac{-p  \sqrt{p^2 - 4q}}{2}}x \\

(r_1 \neq r_2 \not\in \R) \quad r_1 &= a + bi \\
r_2 &= a - bi \\
r_1 + r_2 = 2a &= -p \\
r_1r_2 = a^2 + b^2 &= q \\
a &= -\frac12 p \\
b &= \pm \sqrt{q - \frac14 p^2} \\
y &= C_1e^{(a + bi)x} + C_2e^{a - bi}x \\
&= e^{ax} (C_1 (\cos bx + i \sin (bx)) + C_2 (\cos bx - i \sin (bx))) \\
&= e^{ax} ((C_1 + C_2) \cos bx + i (C_1 - C_2) \sin bx) \\
&= e^{ax} (C_1 \cos bx + C_2 \sin bx) \\
&= e^{-\frac12 px} \left( C_1 \cos \sqrt{q - \frac14 p^2} \, x + C_2 \sin \sqrt{q - \frac14 p^2} \, x \right) \\

y = \begin{cases}
e^{-\frac12 px}(C_1x + C_2) & (\Delta = 0) \\
C_1e^{\frac{-p + \sqrt{p^2 - 4q}}{2}x} + C_2e^{\frac{-p  \sqrt{p^2 - 4q}}{2}}x & (\Delta > 0) \\
e^{-\frac12 px} \left( C_1 \cos \sqrt{q - \frac14 p^2} \, x + C_2 \sin \sqrt{q - \frac14 p^2} \, x \right) & (\Delta < 0)
\end{cases}
\end{align}
$$

